theories/instantiation_func.v
@@ -1,13 +1,13 @@
 (** Executable instantiation **)
 
 From mathcomp Require Import ssreflect ssrbool ssrnat eqtype seq.
-From Wasm Require Import opsem interpreter_func instantiation_spec.
+From Wasm Require Import opsem interpreter_ctx instantiation_spec.
 From Coq Require Import BinNat.
 
 Section Instantiation_func.
 
 Import EmptyHost.
-Import Interpreter_func_extract.
+Import Interpreter_ctx_extract.
 
 Let alloc_funcs := alloc_funcs host_function_eqType.
 Let alloc_tabs := alloc_tabs host_function_eqType.
@@ -20,8 +20,6 @@ Let init_mems := init_mems host_function_eqType.
 
 Let instantiate := instantiate host_function_eqType host_instance.
 Let interp_alloc_module := interp_alloc_module host_function_eqType.
-
-Let run_v := run_v tt.
 
 
 Definition gather_m_f_type (tfs : list function_type) (m_f : module_func) : option function_type :=
